Switch to well-typed expr representation

system-t.v
@@ -1,69 +1,45 @@
-Require Import String.
+Require List.
+Import List.ListNotations.
+Open Scope list.
+
+Set Implicit Arguments.
 
 Inductive type :=
   | natTy
   | arrow : type -> type -> type.
 
-Inductive expr :=
-| var : string -> expr
-| zero : expr
-| succ : expr -> expr
-| iter : forall (ez:expr) (x:string) (e:expr) (n:expr), expr
-| abs : string -> type -> expr -> expr
-| app : expr -> expr -> expr.
+Definition mapping := list type.
 
-Implicit Types (x:string) (t:type) (e:expr).
+Implicit Types (Gamma: mapping) (t: type).
 
-Definition mapping := string -> option type.
+Inductive variable : mapping -> type -> Type :=
+| var_here : forall Gamma t, variable (t :: Gamma) t
+| var_later : forall Gamma t t', variable Gamma t -> variable (t' :: Gamma) t.
 
-Definition upd (m: mapping) v0 t : mapping :=
-  fun v =>
-    if string_dec v v0
-    then Some t
-    else m v.
-
-Theorem upd_eq : forall m v t v',
-    v = v' ->
-    upd m v t v' = Some t.
+Theorem variable_to_in : forall Gamma t,
+    variable Gamma t -> List.In t Gamma.
 Proof.
-  unfold upd; intros.
-  destruct (string_dec v' v); congruence.
+  induction 1; simpl; intros; eauto.
 Qed.
 
-Theorem upd_ne : forall m v t v',
-    v <> v' ->
-    upd m v t v' = m v'.
-Proof.
-  unfold upd; intros.
-  destruct (string_dec v' v); congruence.
-Qed.
+Definition variable_add Gamma t (v: variable Gamma t) t' :
+  variable (t' :: Gamma) t :=
+  var_later t' v.
 
-Inductive hasTy : mapping -> expr -> type -> Prop :=
-| hasTy_var : forall Gamma s t, Gamma s = Some t -> hasTy Gamma (var s) t
-| hasTy_zero : forall Gamma, hasTy Gamma zero natTy
-| hasTy_succ: forall Gamma e, hasTy Gamma e natTy -> hasTy Gamma (succ e) natTy
-| hasTy_iter : forall Gamma e ez t n x,
-    hasTy Gamma ez t -> hasTy Gamma n natTy ->
-    hasTy (upd Gamma x t) e t ->
-    hasTy Gamma (iter ez x e n) t
-| hasTy_lambda : forall Gamma x e t1 t2,
-    hasTy (upd Gamma x t1) e t2 ->
-    hasTy Gamma (abs x t1 e) (arrow t1 t2)
-| hasTy_app : forall Gamma e1 e2 t1 t2,
-    hasTy Gamma e1 (arrow t1 t2) ->
-    hasTy Gamma e2 t1 ->
-    hasTy Gamma (app e1 e2) t2.
-
-Infix "==v" := (string_dec) (at level 30, no associativity).
-
-Fixpoint subst x (x': expr) e : expr :=
-  match e with
-  | var s => if s ==v x then x' else var s
-  | zero => zero
-  | succ e => succ (subst x x' e)
-  | abs v t e => abs v t (if v ==v x then e else subst x x' e)
-  | iter ez v e n => let ez' := subst x x' ez in
-                    let n' := subst x x' n in
-                    iter ez' v (if v ==v x then e else subst x x' e) n'
-  | app e1 e2 => app (subst x x' e1) (subst x x' e1)
-  end.
+Inductive hasTy : mapping -> type -> Type :=
+| var : forall Gamma t (v: variable Gamma t), hasTy Gamma t
+| zero : forall Gamma, hasTy Gamma natTy
+| succ : forall Gamma, hasTy Gamma natTy -> hasTy Gamma natTy
+| abs : forall Gamma t1 (v: variable Gamma t1) t2,
+    forall (e: hasTy (t1 :: Gamma) t2),
+      hasTy Gamma (arrow t1 t2)
+| app : forall Gamma t1 t2,
+    forall (e1: hasTy Gamma (arrow t1 t2))
+      (e2: hasTy Gamma t1),
+      hasTy Gamma t2
+| iter : forall Gamma t,
+    forall (ez: hasTy Gamma t)
+      (v: variable Gamma t)
+      (e: hasTy Gamma t)
+      (n: hasTy Gamma natTy),
+      hasTy Gamma t.
